theories/saturn/inf_ws_deque.v
@@ -33,7 +33,7 @@ From zebre Require Import
 Implicit Types front : nat.
 Implicit Types back : Z.
 Implicit Types l slot : location.
-Implicit Types p : prophecy_id.
+Implicit Types pid : prophet_id.
 Implicit Types id : identifier.
 Implicit Types v t data : val.
 Implicit Types hist model : list val.
@@ -100,7 +100,7 @@ Module raw.
     in_type "t" 2
   )(in custom zebre_field
   ).
-  #[local] Notation "'prophecy'" := (
+  #[local] Notation "'prophet'" := (
     in_type "t" 3
   )(in custom zebre_field
   ).
@@ -121,7 +121,7 @@ Module raw.
       let: "front" := "t".{front} in
       let: "back" := "t".{back} in
       if: "front" < "back" then (
-        if: Resolve (Cas "t".[front] "front" ("front" + #1)) "t".{prophecy} ("front", "id") then (
+        if: Resolve (Cas "t".[front] "front" ("front" + #1)) "t".{prophet} ("front", "id") then (
           ‘Some{ inf_array_get "t".{data} "front" }
         ) else (
           "inf_ws_deque_steal" "t"
@@ -143,7 +143,7 @@ Module raw.
         if: "front" < "back" then (
           ‘Some{ inf_array_get "t".{data} "back" }
         ) else (
-          if: Resolve (Cas "t".[front] "front" ("front" + #1)) "t".{prophecy} ("front", "id") then (
+          if: Resolve (Cas "t".[front] "front" ("front" + #1)) "t".{prophet} ("front", "id") then (
             "t" <-{back} "front" + #1 ;;
             ‘Some{ inf_array_get "t".{data} "back" }
           ) else (
@@ -358,7 +358,7 @@ Module raw.
         /inf_ws_deque_state_inner₃₁
         /inf_ws_deque_state_inner₃₂.
 
-    #[local] Definition inf_ws_deque_inv_inner l γ ι data p : iProp Σ :=
+    #[local] Definition inf_ws_deque_inv_inner l γ ι data pid : iProp Σ :=
       ∃ front back hist model priv past prophs,
       (* mutable physical fields *)
       l.[front] ↦ #front ∗
@@ -373,21 +373,21 @@ Module raw.
       inf_ws_deque_model₁ γ model ∗
       ⌜length model = Z.to_nat (back - front)⌝ ∗
       (* prophet model *)
-      wise_prophet_model inf_ws_deque_prophet p γ.(inf_ws_deque_meta_prophet) past prophs ∗
+      wise_prophet_model inf_ws_deque_prophet pid γ.(inf_ws_deque_meta_prophet) past prophs ∗
       ⌜Forall (λ '(front', _), front' < front) past⌝ ∗
       (* state *)
       inf_ws_deque_state γ ι front back hist model prophs.
     Definition inf_ws_deque_inv t ι : iProp Σ :=
-      ∃ l γ data p,
+      ∃ l γ data pid,
       ⌜t = #l⌝ ∗
       (* metadata *)
       meta l nroot γ ∗
       (* immutable physical fields *)
       l.[data] ↦□ data ∗
-      l.[prophecy] ↦□ #p ∗
+      l.[prophet] ↦□ #pid ∗
       (* invariants *)
       inf_array_inv data ∗
-      inv ι (inf_ws_deque_inv_inner l γ ι data p).
+      inv ι (inf_ws_deque_inv_inner l γ ι data pid).
 
     #[global] Instance inf_ws_deque_model_timeless t model :
       Timeless (inf_ws_deque_model t model).
@@ -734,10 +734,10 @@ Module raw.
       iApply (inf_ws_deque_lock_exclusive with "Hlock1 Hlock2").
     Qed.
 
-    #[local] Lemma inf_ws_deque_wp_get_hist l γ ι data p i v :
+    #[local] Lemma inf_ws_deque_wp_get_hist l γ ι data pid i v :
       {{{
         inf_array_inv data ∗
-        inv ι (inf_ws_deque_inv_inner l γ ι data p) ∗
+        inv ι (inf_ws_deque_inv_inner l γ ι data pid) ∗
         l.[data] ↦□ data ∗
         inf_ws_deque_hist_elem γ i v
       }}}
@@ -780,11 +780,11 @@ Module raw.
       erewrite list_lookup_total_correct; last done.
       iApply ("HΦ" with "[//]").
     Qed.
-    #[local] Lemma inf_ws_deque_wp_get_priv l γ ι data p back priv i :
+    #[local] Lemma inf_ws_deque_wp_get_priv l γ ι data pid back priv i :
       (back ≤ i)%Z →
       {{{
         inf_array_inv data ∗
-        inv ι (inf_ws_deque_inv_inner l γ ι data p) ∗
+        inv ι (inf_ws_deque_inv_inner l γ ι data pid) ∗
         l.[data] ↦□ data ∗
         inf_ws_deque_ctl₂ γ back priv ∗
         inf_ws_deque_lock γ
@@ -841,14 +841,14 @@ Module raw.
       iApply "HΦ". iFrame.
     Qed.
 
-    #[local] Lemma inf_ws_deque_wp_resolve_inconsistent_1 l γ ι data p front id prophs_lb (front1 front2 : Z) :
+    #[local] Lemma inf_ws_deque_wp_resolve_inconsistent_1 l γ ι data pid front id prophs_lb (front1 front2 : Z) :
       head $ filter (λ '(front', _), front' = front) prophs_lb = None →
       {{{
         inf_array_inv data ∗
-        inv ι (inf_ws_deque_inv_inner l γ ι data p) ∗
+        inv ι (inf_ws_deque_inv_inner l γ ι data pid) ∗
         wise_prophet_lb inf_ws_deque_prophet γ.(inf_ws_deque_meta_prophet) prophs_lb
       }}}
-        Resolve (Cas #l.[front] #front1 #front2) #p (#front, #id)%V
+        Resolve (Cas #l.[front] #front1 #front2) #pid (#front, #id)%V
       {{{ v,
         RET v; False
       }}}.
@@ -867,16 +867,16 @@ Module raw.
       all: eelim (filter_nil_not_elem_of _ _ (front, id)); [done.. |].
       all: apply elem_of_app; right; apply elem_of_cons; naive_solver.
     Qed.
-    #[local] Lemma inf_ws_deque_wp_resolve_loser l γ ι data p front _front id id' prophs_lb v :
+    #[local] Lemma inf_ws_deque_wp_resolve_loser l γ ι data pid front _front id id' prophs_lb v :
       head $ filter (λ '(front', _), front' = front) prophs_lb = Some (_front, id') →
       id ≠ id' →
       {{{
         inf_array_inv data ∗
-        inv ι (inf_ws_deque_inv_inner l γ ι data p) ∗
+        inv ι (inf_ws_deque_inv_inner l γ ι data pid) ∗
         inf_ws_deque_front_lb γ front ∗
         wise_prophet_lb inf_ws_deque_prophet γ.(inf_ws_deque_meta_prophet) prophs_lb
       }}}
-        Resolve (Cas #l.[front] #front v) #p (#front, #id)%V
+        Resolve (Cas #l.[front] #front v) #pid (#front, #id)%V
       {{{
         RET #false;
         inf_ws_deque_front_lb γ (S front)
@@ -925,18 +925,18 @@ Module raw.
 
       iApply ("HΦ" with "Hfront_lb").
     Qed.
-    #[local] Lemma inf_ws_deque_wp_resolve_inconsistent_2 l γ ι data p front _front priv Ψ id id' prophs_lb v :
+    #[local] Lemma inf_ws_deque_wp_resolve_inconsistent_2 l γ ι data pid front _front priv Ψ id id' prophs_lb v :
       head $ filter (λ '(front', _), front' = front) prophs_lb = Some (_front, id') →
       id ≠ id' →
       {{{
         inf_array_inv data ∗
-        inv ι (inf_ws_deque_inv_inner l γ ι data p) ∗
+        inv ι (inf_ws_deque_inv_inner l γ ι data pid) ∗
         inf_ws_deque_ctl₂ γ front priv ∗
         inf_ws_deque_front_lb γ front ∗
         wise_prophet_lb inf_ws_deque_prophet γ.(inf_ws_deque_meta_prophet) prophs_lb ∗
         inf_ws_deque_winner₂ γ front Ψ
       }}}
-        Resolve (Cas #l.[front] #front v) #p (#front, #id)%V
+        Resolve (Cas #l.[front] #front v) #pid (#front, #id)%V
       {{{
         RET #false; False
       }}}.
@@ -975,12 +975,12 @@ Module raw.
       wp_apply (inf_array_create_spec with "[//]") as "%data (#Harray_inv & Harray_model)".
 
       (* → [Proph] *)
-      wp_apply (wise_prophet_wp_proph with "[//]") as "%p %γ_prophet %prophs Hprophet_model".
+      wp_apply (wise_prophet_wp_proph with "[//]") as "%pid %γ_prophet %prophs Hprophet_model".
 
-      (* → [{ #0; #0; data; #p }] *)
-      wp_record l as "Hmeta" "(Hfront & Hback & Hdata & Hp & _)".
+      (* → [{ #0; #0; data; #pid }] *)
+      wp_record l as "Hmeta" "(Hfront & Hback & Hdata & Hpid & _)".
       iMod (pointsto_persist with "Hdata") as "#Hdata".
-      iMod (pointsto_persist with "Hp") as "#Hp".
+      iMod (pointsto_persist with "Hpid") as "#Hpid".
 
       iApply "HΦ".
 
@@ -1027,7 +1027,7 @@ Module raw.
         inf_ws_deque_owner t
       >>>.
     Proof.
-      iIntros "!> %Φ ((%l & %γ & %data & %p & -> & #Hmeta & #Hdata & #Hp & #Harray_inv & #Hinv) & (%_l & %_γ & %back & %priv & %Heq & #_Hmeta & Hctl₂ & Hlock)) HΦ". injection Heq as <-.
+      iIntros "!> %Φ ((%l & %γ & %data & %pid & -> & #Hmeta & #Hdata & #Hpid & #Harray_inv & #Hinv) & (%_l & %_γ & %back & %priv & %Heq & #_Hmeta & Hctl₂ & Hlock)) HΦ". injection Heq as <-.
       iDestruct (meta_agree with "Hmeta _Hmeta") as %<-. iClear "_Hmeta".
 
       wp_rec. wp_pures.
@@ -1150,7 +1150,7 @@ Module raw.
       | RET head model; True
       >>>.
     Proof.
-      iIntros "!> %Φ (%l & %γ & %data & %p & -> & #Hmeta & #Hdata & #Hp & #Harray_inv & #Hinv) HΦ".
+      iIntros "!> %Φ (%l & %γ & %data & %pid & -> & #Hmeta & #Hdata & #Hpid & #Harray_inv & #Hinv) HΦ".
       iLöb as "IH".
 
       wp_rec.
@@ -1222,13 +1222,13 @@ Module raw.
         (* → [if: #(bool_decide (front1 < back2))] *)
         rewrite bool_decide_eq_true_2; first done.
 
-        (* → [!#l.[prophecy]] *)
+        (* → [!#l.[prophet]] *)
         wp_load.
 
         wp_pures.
 
-        (* → [Resolve (Cas #l.[front] #front1 #(front1 + 1)) #p (#front1, #id)] *)
-        wp_bind (Resolve (Cas #l.[front] #front1 #(front1 + 1)) #p (#front1, #id)%V).
+        (* → [Resolve (Cas #l.[front] #front1 #(front1 + 1)) #pid (#front1, #id)] *)
+        wp_bind (Resolve (Cas #l.[front] #front1 #(front1 + 1)) #pid (#front1, #id)%V).
         (* open invariant *)
         iInv "Hinv" as "(%front3 & %back3 & %hist & %model & %priv & %past3 & %prophs3 & Hfront & Hback & Hctl₁ & Hfront_auth & Harray_model & Hmodel₁ & >%Hmodel & >Hprophet_model & >%Hpast3 & Hstate)".
         (* do resolve *)
@@ -1286,7 +1286,7 @@ Module raw.
         (* → [if: #(bool_decide (front1 < back2))] *)
         rewrite bool_decide_eq_true_2; first done.
 
-        (* → [!#l.[prophecy]] *)
+        (* → [!#l.[prophet]] *)
         wp_load.
 
         (* inconsistent prophecy resolution *)
@@ -1308,7 +1308,7 @@ Module raw.
         (* → [if: #(bool_decide (front1 < back2))] *)
         rewrite bool_decide_eq_true_2; first done.
 
-        (* → [!#l.[prophecy]] *)
+        (* → [!#l.[prophet]] *)
         wp_load.
 
         (* Cas must fail as we are not the winner *)
@@ -1347,13 +1347,13 @@ Module raw.
       (* → [if: #(bool_decide (front1 < back2))] *)
       rewrite bool_decide_eq_true_2; first done.
 
-      (* → [!#l.[prophecy]] *)
+      (* → [!#l.[prophet]] *)
       wp_load.
 
       wp_pures.
 
-      (* → [Resolve (Cas #l.[front] #front1 #(front1 + 1)) #p (#front1, #id)] *)
-      wp_bind (Resolve (Cas #l.[front] #front1 #(front1 + 1)) #p (#front1, #id)%V).
+      (* → [Resolve (Cas #l.[front] #front1 #(front1 + 1)) #pid (#front1, #id)] *)
+      wp_bind (Resolve (Cas #l.[front] #front1 #(front1 + 1)) #pid (#front1, #id)%V).
       (* open invariant *)
       iInv "Hinv" as "(%front3 & %back3 & %hist & %model & %priv & %past3 & %prophs3 & Hfront & Hback & Hctl₁ & Hfront_auth & Harray_model & Hmodel₁ & >%Hmodel & >Hprophet_model & >%Hpast3 & Hstate)".
       (* we are in state 2 or state 3.1 *)
@@ -1476,7 +1476,7 @@ Module raw.
         inf_ws_deque_owner t
       >>>.
     Proof.
-      iIntros "!> %Φ ((%l & %γ & %data & %p & -> & #Hmeta & #Hdata & #Hp & #Harray_inv & #Hinv) & (%_l & %_γ & %back & %priv & %Heq & #_Hmeta & Hctl₂ & Hlock)) HΦ". injection Heq as <-.
+      iIntros "!> %Φ ((%l & %γ & %data & %pid & -> & #Hmeta & #Hdata & #Hpid & #Harray_inv & #Hinv) & (%_l & %_γ & %back & %priv & %Heq & #_Hmeta & Hctl₂ & Hlock)) HΦ". injection Heq as <-.
       iDestruct (meta_agree with "Hmeta _Hmeta") as %<-. iClear "_Hmeta".
 
       wp_rec.
@@ -1661,13 +1661,13 @@ Module raw.
         + (* → [if: #(bool_decide (front3 < front3))] *)
           rewrite bool_decide_eq_false_2; first lia.
 
-          (* → [!#l.[prophecy]] *)
+          (* → [!#l.[prophet]] *)
           wp_load.
 
           wp_pures.
 
-          (* → [Resolve (Cas #l.[front] #front3 #(front3 + 1)) #p (#front3, #id)] *)
-          wp_bind (Resolve (Cas #l.[front] #front3 #(front3 + 1)) #p (#front3, #id)%V).
+          (* → [Resolve (Cas #l.[front] #front3 #(front3 + 1)) #pid (#front3, #id)] *)
+          wp_bind (Resolve (Cas #l.[front] #front3 #(front3 + 1)) #pid (#front3, #id)%V).
           (* open invariant *)
           iInv "Hinv" as "(%front4 & %_back & %hist & %model & %_priv & %past4 & %prophs4 & Hfront & Hback & >Hctl₁ & >Hfront_auth & Harray_model & Hmodel₁ & >%Hmodel & >Hprophet_model & >%Hpast4 & Hstate)".
           iDestruct (inf_ws_deque_ctl_agree with "Hctl₁ Hctl₂") as %(-> & ->).
@@ -1813,7 +1813,7 @@ Module raw.
           (* → [if: #(bool_decide (front2 < front2))] *)
           rewrite bool_decide_eq_false_2; first lia.
 
-          (* → [!#l.[prophecy]] *)
+          (* → [!#l.[prophet]] *)
           wp_load.
 
           (* inconsistent prophecy resolution *)
@@ -1877,13 +1877,13 @@ Module raw.
           (* → [if: #(bool_decide (front2 < front2))] *)
           rewrite bool_decide_eq_false_2; first lia.
 
-          (* → [!#l.[prophecy]] *)
+          (* → [!#l.[prophet]] *)
           wp_load.
 
           wp_pures.
 
-          (* → [Resolve (Cas #l.[front] #front2 #(front2 + 1)) #p (#front2, #id)] *)
-          wp_bind (Resolve (Cas #l.[front] #front2 #(front2 + 1)) #p (#front2, #id)%V).
+          (* → [Resolve (Cas #l.[front] #front2 #(front2 + 1)) #pid (#front2, #id)] *)
+          wp_bind (Resolve (Cas #l.[front] #front2 #(front2 + 1)) #pid (#front2, #id)%V).
           (* open invariant *)
           iInv "Hinv" as "(%front4 & %_back & %hist & %model & %_priv & %past4 & %prophs4 & Hfront & Hback & >Hctl₁ & Hfront_auth & Harray_model & Hmodel₁ & >%Hmodel & >Hprophet_model & >%Hpast4 & Hstate)".
           iDestruct (inf_ws_deque_ctl_agree with "Hctl₁ Hctl₂") as %(-> & ->).
@@ -2001,7 +2001,7 @@ Module raw.
             (* → [if: #(bool_decide (front2 < front2))] *)
             rewrite bool_decide_eq_false_2; first lia.
 
-            (* → [!#l.[prophecy]] *)
+            (* → [!#l.[prophet]] *)
             wp_load.
 
             (* inconsistent prophecy resolution *)
@@ -2080,7 +2080,7 @@ Module raw.
                 (* → [if: #(bool_decide (front2 < front2))] *)
                 rewrite bool_decide_eq_false_2; first lia.
 
-                (* → [!#l.[prophecy]] *)
+                (* → [!#l.[prophet]] *)
                 wp_load.
 
                 (* Cas must fail as we are not the winner *)
