theories/iris/base_logic/lib/prophet_map.v
@@ -1,0 +1,145 @@
+From iris.base_logic.lib Require Import
+  ghost_map.
+
+From zebre Require Import
+  prelude.
+From zebre.iris.base_logic Require Export
+  lib.base.
+From zebre.iris Require Import
+  diaframe.
+From zebre Require Import
+  options.
+
+Class ProphetMapGpre Σ P V `{Countable P} := {
+  #[local] prophet_map_Gpre_inG :: ghost_mapG Σ P (list V) ;
+}.
+
+Class ProphetMapG Σ P V `{Countable P} := {
+  #[local] prophet_map_inG :: ProphetMapGpre Σ P V ;
+  prophet_map_name : gname ;
+}.
+#[global] Arguments prophet_map_name {_ _ _ _ _} _ : assert.
+
+Definition prophet_map_Σ P V `{Countable P} :=
+  ghost_mapΣ P (list V).
+#[global] Instance subG_prophet_map_Σ Σ P V `{Countable P} :
+  subG (prophet_map_Σ P V) Σ →
+  ProphetMapGpre Σ P V.
+Proof.
+  solve_inG.
+Qed.
+
+Section prophecies_resolve.
+  Context {P V : Type} `{Countable P}.
+
+  Implicit Type pid : P.
+  Implicit Type prophets : gmap P (list V).
+
+  Fixpoint prophecies_resolve xprophs pid : list V :=
+    match xprophs with
+    | [] =>
+        []
+    | xproph :: xprophs =>
+        if decide (pid = xproph.1) then
+          xproph.2 :: prophecies_resolve xprophs pid
+        else
+          prophecies_resolve xprophs pid
+    end.
+
+  Definition prophets_resolve prophets xprophs :=
+    map_Forall (λ pid prophs, prophs = prophecies_resolve xprophs pid) prophets.
+
+  Lemma resolves_insert xprophs pid prophets :
+    prophets_resolve prophets xprophs →
+    pid ∉ dom prophets →
+    prophets_resolve (<[pid := prophecies_resolve xprophs pid]> prophets) xprophs.
+  Proof.
+    intros Hinlist Hpid pid' prophs Hlookup.
+    destruct (decide (pid = pid')) as [-> | Hne].
+    - rewrite lookup_insert in Hlookup.
+      inversion Hlookup. done.
+    - rewrite lookup_insert_ne // in Hlookup.
+      apply Hinlist. done.
+  Qed.
+End prophecies_resolve.
+
+Section prophet_map_G.
+  Context `{prophet_map_G : ProphetMapG Σ P V}.
+
+  Definition prophet_map_interp xprophs pids : iProp Σ :=
+    ∃ prophets,
+    ⌜prophets_resolve prophets xprophs ∧ dom prophets ⊆ pids⌝ ∗
+    ghost_map_auth prophet_map_G.(prophet_map_name) 1 prophets.
+
+  Definition prophet_model pid prophs : iProp Σ :=
+    ghost_map_elem prophet_map_G.(prophet_map_name) pid (DfracOwn 1) prophs.
+
+  #[global] Instance prophet_model_timeless pid prophs :
+    Timeless (prophet_model pid prophs).
+  Proof.
+    apply _.
+  Qed.
+
+  Lemma prophet_model_exclusive pid prophs1 prophs2 :
+    prophet_model pid prophs1 -∗
+    prophet_model pid prophs2 -∗
+    False.
+  Proof.
+    iIntros "Hmodel1 Hmodel2".
+    iDestruct (ghost_map_elem_ne with "Hmodel1 Hmodel2") as %?.
+    iSteps.
+  Qed.
+
+  Lemma prophet_map_new pid pids xprophs :
+    pid ∉ pids →
+    prophet_map_interp xprophs pids ==∗
+      prophet_map_interp xprophs ({[pid]} ∪ pids) ∗
+      prophet_model pid (prophecies_resolve xprophs pid).
+  Proof.
+    iIntros "%Hpid Hpids".
+    iDestruct "Hpids" as "(%prophets & (%Hprophets & %Hpids) & Hauth)".
+    iMod (ghost_map_insert pid (prophecies_resolve xprophs pid) with "Hauth") as "(Hauth & Helem)".
+    { apply not_elem_of_dom. set_solver. }
+    iModIntro. iFrame. iExists (<[pid := prophecies_resolve xprophs pid]> prophets). iFrame. iPureIntro.
+    split.
+    - apply resolves_insert; first done. set_solver.
+    - rewrite dom_insert. set_solver.
+  Qed.
+
+  Lemma prophet_map_resolve pid proph xprophs pids prophs :
+    prophet_map_interp ((pid, proph) :: xprophs) pids -∗
+    prophet_model pid prophs ==∗
+      ∃ prophs',
+      ⌜prophs = proph :: prophs'⌝ ∗
+      prophet_map_interp xprophs pids ∗
+      prophet_model pid prophs'.
+  Proof.
+    iIntros "Hpids Hp".
+    iDestruct "Hpids" as "(%prophets & (%Hprophets & %Hpids) & Hauth)".
+    iCombine "Hauth Hp" gives %Hlookup.
+    assert (prophs = proph :: prophecies_resolve xprophs pid) as ->.
+    { rewrite (Hprophets pid prophs Hlookup) /= decide_True //. }
+    iMod (ghost_map_update (prophecies_resolve xprophs pid) with "Hauth Hp") as "(Hauth & Helem)".
+    iExists (prophecies_resolve xprophs pid). iFrame. iSplitR; first iSteps.
+    iExists _. iFrame. iPureIntro. split.
+    - intros pid' prophs' Hlookup'. destruct (decide (pid = pid')) as [<- | Hne].
+      + rewrite lookup_insert in Hlookup'.
+        inversion Hlookup'. done.
+      + rewrite lookup_insert_ne // in Hlookup'.
+        rewrite (Hprophets pid' prophs' Hlookup') /= decide_False //.
+    - assert (pid ∈ dom prophets) by exact: elem_of_dom_2.
+      rewrite dom_insert. set_solver.
+  Qed.
+End prophet_map_G.
+
+Lemma prophet_map_init `{prophet_map_Gpre : ProphetMapGpre Σ P V} xprophs pids :
+  ⊢ |==>
+    ∃ _ : ProphetMapG Σ P V,
+    prophet_map_interp xprophs pids.
+Proof.
+  iMod (ghost_map_alloc_empty) as (γ) "Hauth".
+  iExists (Build_ProphetMapG _ _ _ _ _ _ _), ∅. iSteps.
+Qed.
+
+#[global] Opaque prophet_map_interp.
+#[global] Opaque prophet_model.
